Upgrade Iris
- Ran the recommended sed script in the Iris CHANGELOG due to the C->O
  suffix rename upstream.
- Reversed rewrite direction of a few *_op lemmas (pair_op, Cinl_op,
  Cinr_op) due to upstream reversal of those equalities:
  https://gitlab.mpi-sws.org/iris/iris/merge_requests/295#note_39151.
- Updated references to fupd_big_sepM and fupd_big_sepS due to upstream
  rename to fupd_big_sep{L,M,S,MS}.

src/CSL/Count_GHeap.v
@@ -11,9 +11,9 @@ Set Default Proof Using "Type".
 Import uPred.
 
 Definition gen_heapUR (L V : Type) `{Countable L} : ucmraT :=
-  gmapUR L (prodR countingR (agreeR (leibnizC V))).
+  gmapUR L (prodR countingR (agreeR (leibnizO V))).
 Definition to_gen_heap {L V} `{Countable L} : gmap L V → gen_heapUR L V :=
-  fmap (λ v, (Count 0, to_agree (v : leibnizC V))).
+  fmap (λ v, (Count 0, to_agree (v : leibnizO V))).
 
 (** The CMRA we need. *)
 Class gen_heapG (L V : Type) (Σ : gFunctors) `{Countable L} := GenHeapG {
@@ -39,13 +39,13 @@ Section definitions.
     own (gen_heap_name hG) (● (to_gen_heap σ)).
 
   Definition mapsto_def (l : L) (n: Z) (v: V) : iProp Σ :=
-    own (gen_heap_name hG) (◯ {[ l := (Count n, to_agree (v : leibnizC V)) ]}).
+    own (gen_heap_name hG) (◯ {[ l := (Count n, to_agree (v : leibnizO V)) ]}).
   Definition mapsto_aux : seal (@mapsto_def). by eexists. Qed.
   Definition mapsto := mapsto_aux.(unseal).
   Definition mapsto_eq : @mapsto = @mapsto_def := mapsto_aux.(seal_eq).
 
   Definition read_mapsto_def (l : L) (v: V) : iProp Σ :=
-    own (gen_heap_name hG) (◯ {[ l := (Count (-1), to_agree (v : leibnizC V)) ]}).
+    own (gen_heap_name hG) (◯ {[ l := (Count (-1), to_agree (v : leibnizO V)) ]}).
   Definition read_mapsto_aux : seal (@read_mapsto_def). by eexists. Qed.
   Definition read_mapsto := read_mapsto_aux.(unseal).
   Definition read_mapsto_eq : @read_mapsto = @read_mapsto_def := read_mapsto_aux.(seal_eq).
@@ -81,7 +81,7 @@ Section to_gen_heap.
     move=> /Some_pair_included_total_2 [_] /to_agree_included /leibniz_equiv_iff -> //.
   Qed.
   Lemma to_gen_heap_insert l v σ :
-    to_gen_heap (<[l:=v]> σ) = <[l:=(Count 0, to_agree (v:leibnizC V))]> (to_gen_heap σ).
+    to_gen_heap (<[l:=v]> σ) = <[l:=(Count 0, to_agree (v:leibnizO V))]> (to_gen_heap σ).
   Proof. by rewrite /to_gen_heap fmap_insert. Qed.
   Lemma to_gen_heap_delete l σ :
     to_gen_heap (delete l σ) = delete l (to_gen_heap σ).
@@ -144,7 +144,7 @@ Section gen_heap.
     apply wand_intro_r.
     rewrite mapsto_eq /mapsto_def.
     rewrite -own_op -auth_frag_op own_valid discrete_valid.
-    f_equiv=> /auth_frag_proj_valid /=. rewrite op_singleton singleton_valid pair_op.
+    f_equiv=> /auth_frag_proj_valid /=. rewrite op_singleton singleton_valid -pair_op.
     by intros [_ ?%agree_op_invL'].
   Qed.
 
@@ -155,7 +155,7 @@ Section gen_heap.
     apply wand_intro_r.
     rewrite mapsto_eq /mapsto_def.
     rewrite -own_op -auth_frag_op own_valid discrete_valid.
-    f_equiv=> /auth_frag_proj_valid /=. rewrite op_singleton singleton_valid pair_op.
+    f_equiv=> /auth_frag_proj_valid /=. rewrite op_singleton singleton_valid -pair_op.
     intros [Hcount ?].
     rewrite counting_op' //= in Hcount.
     repeat destruct decide => //=. lia.
@@ -165,7 +165,7 @@ Section gen_heap.
   Proof.
     rewrite mapsto_eq /mapsto_def.
     rewrite -own_op -auth_frag_op.
-    rewrite op_singleton pair_op.
+    rewrite op_singleton -pair_op.
     rewrite counting_op' //=.
     repeat destruct decide => //=. lia.
     replace (S q + (-1))%Z with (q : Z) by lia.
@@ -178,7 +178,7 @@ Section gen_heap.
     iIntros (?) "Hσ". rewrite /gen_heap_ctx mapsto_eq /mapsto_def.
     iMod (own_update with "Hσ") as "[Hσ Hl]".
     { eapply auth_update_alloc,
-        (alloc_singleton_local_update _ _ (Count 0, to_agree (v:leibnizC _)))=> //.
+        (alloc_singleton_local_update _ _ (Count 0, to_agree (v:leibnizO _)))=> //.
       by apply lookup_to_gen_heap_None. }
     iModIntro. rewrite to_gen_heap_insert. iFrame.
   Qed.
@@ -213,7 +213,7 @@ Section gen_heap.
       as %[Hl%gen_heap_singleton_included _]%auth_both_valid.
     iMod (own_update_2 with "Hσ Hl") as "[Hσ Hl]".
     { eapply auth_update, singleton_local_update,
-        (exclusive_local_update _ (Count 0, to_agree (v2:leibnizC _)))=> //.
+        (exclusive_local_update _ (Count 0, to_agree (v2:leibnizO _)))=> //.
       by rewrite /to_gen_heap lookup_fmap Hl. }
     iModIntro. rewrite to_gen_heap_insert. iFrame.
   Qed.
