src/Examples/ExMach/Adequacy.v
@@ -10,11 +10,11 @@ Class exmachPreG Σ := ExMachPreG {
   exm_preG_iris :> invPreG Σ;
   exm_preG_mem :> gen_heapPreG nat nat Σ;
   exm_preG_disk :> leased_heapPreG nat nat Σ;
-  exm_preG_treg_inG :> inG Σ (csumR countingR (authR (optionUR (exclR unitC))));
+  exm_preG_treg_inG :> inG Σ (csumR countingR (authR (optionUR (exclR unitO))));
 }.
 
 Definition exmachΣ : gFunctors := #[invΣ; gen_heapΣ nat nat; leased_heapΣ nat nat;
-                                    GFunctor (csumR countingR (authR (optionUR (exclR unitC))))].
+                                    GFunctor (csumR countingR (authR (optionUR (exclR unitO))))].
 Instance subG_exmachPreG {Σ} : subG exmachΣ Σ → exmachPreG Σ.
 Proof. solve_inG. Qed.
 
