src/Examples/ExMach/RefinementAdequacy.v
@@ -19,7 +19,7 @@ Module Type exmach_refinement_type.
   Notation compile_proc_seq := (compile_proc_seq impl).
   Context `{CFG: cfgPreG OpT Λa Σ} `{HEX: exmachPreG Σ}.
   Context `{INV: Adequacy.invPreG Σ}.
-  Context `{REG: inG Σ (csumR countingR (authR (optionUR (exclR unitC))))}.
+  Context `{REG: inG Σ (csumR countingR (authR (optionUR (exclR unitO))))}.
   Context (crash_inner: forall {_ : @cfgG OpT Λa Σ} {_: exmachG Σ}, iProp Σ).
   Context (exec_inner: forall {_ : @cfgG OpT Λa Σ} {_: exmachG Σ}, iProp Σ).
   Context (crash_param: forall (_ : @cfgG OpT Λa Σ) (_ : exmachG Σ), Type).
