src/Examples/ExMach/WeakestPre.v
@@ -400,8 +400,8 @@ End lifting.
    except we don't allocate locks or pass the pointer to them; there is a dedicated
    lock register. *)
 
-Class lockG Σ := LockG { lock_tokG :> inG Σ (exclR unitC) }.
-Definition lockΣ : gFunctors := #[GFunctor (exclR unitC)].
+Class lockG Σ := LockG { lock_tokG :> inG Σ (exclR unitO) }.
+Definition lockΣ : gFunctors := #[GFunctor (exclR unitO)].
 Instance subG_lockΣ {Σ} : subG lockΣ Σ → lockG Σ.
 Proof. solve_inG. Qed.
 
